skeleton

src/Model/Bernoulli.dfy
@@ -6,18 +6,20 @@
 include "Monad.dfy"
 include "RandomNumberGenerator.dfy"
 include "Independence.dfy"
+include "Uniform.dfy"
 
 module Bernoulli {
   import opened Monad
   import opened RandomNumberGenerator
   import opened Independence
+  import opened Uniform
 
   /************
    Definitions  
   ************/
 
   type Probability = x: real | 0.0 <= x <= 1.0
-
+ 
   // Equation (4.23)
   function ProbBernoulli(p: Probability): Hurd<bool> {
     assume {:axiom} false;
@@ -36,9 +38,84 @@ module Bernoulli {
     Bind(Deconstruct, f)
   }  
 
+  // Footnote 5, p. 82
+  function ProbBernoulliRational(m: nat, n: nat): Hurd<bool> 
+    requires n != 0
+    requires m <= n
+  {
+    Bind(ProbUniform(n), (k: nat) => Return(k < m))
+  }
+
   /*******
    Lemmas  
   *******/
+
+  lemma ProbBernoulliRationalIsIndepFn(m: nat, n: nat)
+    requires n != 0
+    requires m <= n
+    ensures IsIndepFn(ProbBernoulliRational(m, n))
+  {
+    var f := ProbUniform(n);
+    var g := (k: nat) => Return(k < m);
+
+    assert IsIndepFn(f) by {
+      ProbUniformIsIndepFn(n);
+    }
+
+    assert forall k: nat :: IsIndepFn(g(k)) by {
+      forall k: nat ensures IsIndepFn(g(k)) {
+        ReturnIsIndepFn(k < m);
+      }
+    }
+
+    IndepFnIsCompositional(f, g);
+  }
+
+  lemma BernoulliRationalCorrectness(m: nat, n: nat)
+    requires n != 0
+    requires m <= n
+    ensures
+      var e := iset s | ProbBernoulliRational(m, n)(s).0;
+      && e in event_space
+      && mu(e) == m as real / n as real
+  {
+    var e := iset s | ProbBernoulliRational(m, n)(s).0;
+    var e1 := iset s | ProbUniform(n)(s).0 == m-1;
+
+    assert m - 1 <= m <= n;
+    var e2 := iset s | ProbBernoulliRational(m-1, n)(s).0;
+
+    calc {
+      e;
+      iset s | ProbUniform(n)(s).0 < m;
+      iset s | ProbUniform(n)(s).0 == m-1 || ProbUniform(n)(s).0 < m-1;
+      (iset s | ProbUniform(n)(s).0 == m-1) + (iset s | ProbUniform(n)(s).0 < m-1);
+    }
+
+    assume {:axiom} false;
+
+/*     assert (iset s | ProbUniform(n)(s).0 == m-1) == e1;
+    assert (iset s | ProbUniform(n)(s).0 < m-1) == e2;
+    
+    assert mu(e1) == 1.0 / (n as real) by {
+      UniformFullCorrectness(n, m-1);
+    }
+
+    assert mu(e2) == (m - 1) as real / n as real by {
+      BernoulliRationalCorrectness(m-1, n);
+    }
+
+    calc {
+      mu(e);
+      mu(e1 + e2);
+      { assert e1 * e2 == iset{}; }
+      mu(e1) + mu(e2);
+      (1.0 / (n as real)) + ((m-1) as real / n as real);
+      (1.0 + ((m-1) as real)) / n as real;
+      (1.0 + (m as real) - 1.0) / n as real;
+      m as real / n as real;
+    }  */
+  }
 
   lemma {:axiom} ProbBernoulliIsIndepFn(p: Probability)
     ensures IsIndepFn(ProbBernoulli(p))
@@ -48,7 +125,5 @@ module Bernoulli {
       var e := iset s | ProbBernoulli(p)(s).0;
       && e in event_space
       && mu(e) == p
-  
-
 }
 
